more varint work

Varint.go
@@ -1,0 +1,31 @@
+package main
+
+import (
+	"encoding/hex"
+	"fmt"
+	"math"
+	"strconv"
+)
+
+func encode(x uint64) []byte {
+	length := uint64(math.Log2(float64(x))) / 7
+	fmt.Println("Length: ", length)
+	result := make([]byte, 0, length)
+	for x != 0 {
+		nextByte := byte(x & 0x7F)
+		fmt.Println("Extracted: ", nextByte)
+		x = x >> 7
+		// Set continuation bit
+		if x > 0 {
+			nextByte = nextByte | 0x80
+		}
+		fmt.Println("Remaining: ", x)
+		result = append(result, nextByte)
+	}
+	return result
+}
+
+func main() {
+	fmt.Println(strconv.FormatInt(0x7F, 2))
+	fmt.Println(hex.EncodeToString(encode(150)))
+}
